src/program_proof/tulip/program/backup/bgcoord_receive.v
@@ -1,0 +1,44 @@
+From Perennial.program_proof.tulip.program Require Import prelude.
+From Perennial.program_proof.tulip.program.backup Require Import
+  bgcoord_repr bgpreparer_repr.
+
+Section program.
+  Context `{!heapGS Σ, !tulip_ghostG Σ}.
+
+  Theorem wp_BackupGroupCoordinator__Receive
+    (gcoord : loc) (rid : u64) (addrm : gmap u64 chan) (addr : chan) rk ts gid γ :
+    addrm !! rid = Some addr ->
+    is_backup_gcoord_with_addrm gcoord addrm rk ts gid γ -∗
+    {{{ True }}}
+      BackupGroupCoordinator__Receive #gcoord #rid
+    {{{ (dataP : Slice.t) (ok : bool), RET (to_val dataP, #ok);
+        if ok
+        then ∃ (data : list u8) (resp : txnresp),
+            own_slice dataP byteT (DfracOwn 1) data ∗
+            safe_txnresp γ gid resp ∗
+            ⌜encode_txnresp resp data⌝
+        else True
+    }}}.
+  Proof.
+    iIntros (Haddr) "#Hpx".
+    iIntros (Φ) "!> _ HΦ".
+    wp_rec.
+
+    (*@ func (gcoord *BackupGroupCoordinator) Receive(rid uint64) ([]byte, bool) { @*)
+    (*@     conn, ok := gcoord.GetConnection(rid)                               @*)
+    (*@     if !ok {                                                            @*)
+    (*@         gcoord.Connect(rid)                                             @*)
+    (*@         return nil, false                                               @*)
+    (*@     }                                                                   @*)
+    (*@                                                                         @*)
+    (*@     ret := grove_ffi.Receive(conn)                                      @*)
+    (*@     if ret.Err {                                                        @*)
+    (*@         gcoord.Connect(rid)                                             @*)
+    (*@         return nil, false                                               @*)
+    (*@     }                                                                   @*)
+    (*@                                                                         @*)
+    (*@     return ret.Data, true                                               @*)
+    (*@ }                                                                       @*)
+  Admitted.
+
+End program.
