src/program_proof/tulip/program/backup/bgcoord_response_session.v
@@ -1,0 +1,367 @@
+From Perennial.program_proof.tulip.program Require Import prelude.
+From Perennial.program_proof.tulip.program.gcoord Require Import decode.
+From Perennial.program_proof.tulip.program.backup Require Import
+  bgcoord_repr bgpreparer_repr bgcoord_receive
+  bgpreparer_process_inquire_result bgpreparer_process_validate_result
+  bgpreparer_process_prepare_result bgpreparer_process_unprepare_result
+  bgpreparer_process_finalization_result.
+
+Section program.
+  Context `{!heapGS Σ, !tulip_ghostG Σ}.
+
+  Theorem wp_BackupGroupCoordinator__ResponseSession
+    (gcoord : loc) (rid : u64) (addr : chan) (addrm : gmap u64 chan) rk ts gid γ :
+    addrm !! rid = Some addr ->
+    is_backup_gcoord_with_addrm gcoord addrm rk ts gid γ -∗
+    {{{ True }}}
+      BackupGroupCoordinator__ResponseSession #gcoord #rid
+    {{{ RET #(); True }}}.
+  Proof.
+    iIntros (Haddr) "#Hgcoord".
+    iIntros (Φ) "!> _ HΦ".
+    wp_rec.
+    
+
+    (*@ func (gcoord *BackupGroupCoordinator) ResponseSession(rid uint64) {     @*)
+    (*@     for {                                                               @*)
+    (*@                                                                         @*)
+    wp_apply (wp_forBreak (λ _, True)%I); wp_pures; last by iApply "HΦ".
+    clear Φ.
+    iIntros (Φ) "!> _ HΦ".
+    wp_pures.
+
+    (*@         data, ok := gcoord.Receive(rid)                                 @*)
+    (*@         if !ok {                                                        @*)
+    (*@             // Try to re-establish a connection on failure.             @*)
+    (*@             primitive.Sleep(params.NS_RECONNECT)                        @*)
+    (*@             continue                                                    @*)
+    (*@         }                                                               @*)
+    (*@                                                                         @*)
+    wp_apply (wp_BackupGroupCoordinator__Receive with "Hgcoord").
+    { apply Haddr. }
+    iIntros (dataP ok) "Hdata".
+    wp_pures.
+    destruct ok; wp_pures; last first.
+    { wp_apply wp_Sleep.
+      wp_pures.
+      by iApply "HΦ".
+    }
+    iDestruct "Hdata" as (data resp) "(Hdata & #Hresp & %Hdataenc)".
+
+    (*@         msg := message.DecodeTxnResponse(data)                          @*)
+    (*@         kind := msg.Kind                                                @*)
+    (*@                                                                         @*)
+    iDestruct (own_slice_to_small with "Hdata") as "Hdata".
+    wp_apply (wp_DecodeTxnResponse with "Hdata").
+    { apply Hdataenc. }
+    iIntros (pwrsP) "Hpwrs".
+    wp_pures.
+
+    (*@         if gcoord.ts != msg.Timestamp {                                 @*)
+    (*@             continue                                                    @*)
+    (*@         }                                                               @*)
+    (*@         gcoord.mu.Lock()                                                @*)
+    (*@         gpp := gcoord.gpp                                               @*)
+    (*@         if kind == message.MSG_TXN_INQUIRE {                            @*)
+    (*@             // This is a proof artifact since any message received in this @*)
+    (*@             // session should be delivered to @gcoord.cid.              @*)
+    (*@             if gcoord.cid == msg.CoordID {                              @*)
+    (*@                 pp := tulip.PrepareProposal{                            @*)
+    (*@                     Rank     : msg.Rank,                                @*)
+    (*@                     Prepared : msg.Prepared,                            @*)
+    (*@                 }                                                       @*)
+    (*@                 gpp.processInquireResult(msg.ReplicaID, pp, msg.Validated, msg.PartialWrites, msg.Result) @*)
+    (*@             }                                                           @*)
+    (*@         } else if kind == message.MSG_TXN_VALIDATE {                    @*)
+    (*@             gpp.processValidateResult(msg.ReplicaID, msg.Result)        @*)
+    (*@         } else if kind == message.MSG_TXN_PREPARE {                     @*)
+    (*@             gpp.processPrepareResult(msg.ReplicaID, msg.Result)         @*)
+    (*@         } else if kind == message.MSG_TXN_UNPREPARE {                   @*)
+    (*@             gpp.processUnprepareResult(msg.ReplicaID, msg.Result)       @*)
+    (*@         } else if kind == message.MSG_TXN_REFRESH {                     @*)
+    (*@             // No reponse message for REFRESH.                          @*)
+    (*@         } else if kind == message.MSG_TXN_COMMIT || kind == message.MSG_TXN_ABORT { @*)
+    (*@             // Not using msg.Timestamp might be an issue in the proof without an @*)
+    (*@             // invariant saying that message sent through this connection can @*)
+    (*@             // only be of that of the transaction we're finalizing here. @*)
+    (*@             gpp.processFinalizationResult(msg.Result)                   @*)
+    (*@         }                                                               @*)
+    (*@         // In the current design the coordinator will be notified whenever a new @*)
+    (*@         // response arrives, and then checks whether the final result (e.g., @*)
+    (*@         // prepared, committed, or aborted in the case of preparing) is @*)
+    (*@         // ready. An optimization would be requiring those @process{X}Result @*)
+    (*@         // functions to return a bool indicating the final result is ready, and @*)
+    (*@         // call @gcoord.cv.Signal only on those occasions.              @*)
+    (*@         gcoord.cv.Signal()                                              @*)
+    (*@         gcoord.mu.Unlock()                                              @*)
+    (*@     }                                                                   @*)
+    (*@ }                                                                       @*)
+    clear Haddr rid.
+    destruct resp; wp_pures.
+    { (* Case: Read. *)
+      iNamed "Hgcoord".
+      wp_loadField.
+      wp_pures.
+      case_bool_decide as Htseq; wp_pures; last by iApply "HΦ".
+      symmetry in Htseq. inv Htseq.
+      wp_loadField.
+      wp_apply (wp_Mutex__Lock with "Hlock").
+      iIntros "[Hlocked Hgcoord]".
+      iNamed "Hgcoord". iNamed "Hgpp".
+      wp_loadField.
+      wp_pures.
+      wp_loadField.
+      wp_apply (wp_Cond__Signal with "Hcv").
+      wp_loadField.
+      wp_apply (wp_Mutex__Unlock with "[-HΦ]").
+      { by iFrame "Hlock Hlocked ∗". }
+      wp_pures.
+      by iApply "HΦ".
+    }
+    { (* Case: FastPrepare. *)
+      iNamed "Hgcoord".
+      wp_loadField.
+      wp_pures.
+      case_bool_decide as Htseq; wp_pures; last by iApply "HΦ".
+      symmetry in Htseq. inv Htseq.
+      wp_loadField.
+      wp_apply (wp_Mutex__Lock with "Hlock").
+      iIntros "[Hlocked Hgcoord]".
+      iNamed "Hgcoord". iNamed "Hgpp".
+      wp_loadField.
+      wp_pures.
+      wp_loadField.
+      wp_apply (wp_Cond__Signal with "Hcv").
+      wp_loadField.
+      wp_apply (wp_Mutex__Unlock with "[-HΦ]").
+      { by iFrame "Hlock Hlocked ∗". }
+      wp_pures.
+      by iApply "HΦ".
+    }
+    { (* Case: Validate. *)
+      iNamed "Hgcoord".
+      wp_loadField.
+      wp_pures.
+      case_bool_decide as Htseq; wp_pures; last by iApply "HΦ".
+      symmetry in Htseq. inv Htseq.
+      wp_loadField.
+      wp_apply (wp_Mutex__Lock with "Hlock").
+      iIntros "[Hlocked Hgcoord]".
+      iNamed "Hgcoord". iNamed "Hgpp".
+      wp_loadField.
+      wp_pures.
+      iNamed "Hresp".
+      wp_apply (wp_BackupGroupPreparer__processValidateResult with "Hsafe Hinv Hgpp").
+      { apply Hrk. }
+      { apply Hrid. }
+      { apply Hgid. }
+      iIntros "Hgpp".
+      wp_loadField.
+      wp_apply (wp_Cond__Signal with "Hcv").
+      wp_loadField.
+      wp_apply (wp_Mutex__Unlock with "[-HΦ]").
+      { by iFrame "Hlock Hlocked ∗". }
+      wp_pures.
+      by iApply "HΦ".
+    }
+    { (* Case: Prepare. *)
+      iNamed "Hgcoord".
+      wp_loadField.
+      wp_pures.
+      case_bool_decide as Htseq; wp_pures; last by iApply "HΦ".
+      symmetry in Htseq. inv Htseq.
+      wp_loadField.
+      wp_apply (wp_Mutex__Lock with "Hlock").
+      iIntros "[Hlocked Hgcoord]".
+      iNamed "Hgcoord". iNamed "Hgpp".
+      wp_loadField.
+      wp_pures.
+      wp_loadField.
+      wp_pures.
+      case_bool_decide as Hrank; wp_pures.
+      { inv Hrank.
+        iNamed "Hresp".
+        wp_apply (wp_BackupGroupPreparer__processPrepareResult with "Hsafe Hgpp").
+        { apply Hrk. }
+        { apply Hrid. }
+        iIntros "Hgpp".
+        wp_loadField.
+        wp_apply (wp_Cond__Signal with "Hcv").
+        wp_loadField.
+        wp_apply (wp_Mutex__Unlock with "[-HΦ]").
+        { by iFrame "Hlock Hlocked ∗". }
+        wp_pures.
+        by iApply "HΦ".
+      }
+      wp_loadField.
+      wp_apply (wp_Cond__Signal with "Hcv").
+      wp_loadField.
+      wp_apply (wp_Mutex__Unlock with "[-HΦ]").
+      { by iFrame "Hlock Hlocked ∗". }
+      wp_pures.
+      by iApply "HΦ".
+    }
+    { (* Case: Unprepare. *)
+      iNamed "Hgcoord".
+      wp_loadField.
+      wp_pures.
+      case_bool_decide as Htseq; wp_pures; last by iApply "HΦ".
+      symmetry in Htseq. inv Htseq.
+      wp_loadField.
+      wp_apply (wp_Mutex__Lock with "Hlock").
+      iIntros "[Hlocked Hgcoord]".
+      iNamed "Hgcoord". iNamed "Hgpp".
+      wp_loadField.
+      wp_pures.
+      wp_loadField.
+      wp_pures.
+      case_bool_decide as Hrank; wp_pures.
+      { inv Hrank.
+        iNamed "Hresp".
+        wp_apply (wp_BackupGroupPreparer__processUnprepareResult with "Hsafe Hgpp").
+        { apply Hrk. }
+        { apply Hrid. }
+        iIntros "Hgpp".
+        wp_loadField.
+        wp_apply (wp_Cond__Signal with "Hcv").
+        wp_loadField.
+        wp_apply (wp_Mutex__Unlock with "[-HΦ]").
+        { by iFrame "Hlock Hlocked ∗". }
+        wp_pures.
+        by iApply "HΦ".
+      }
+      wp_loadField.
+      wp_apply (wp_Cond__Signal with "Hcv").
+      wp_loadField.
+      wp_apply (wp_Mutex__Unlock with "[-HΦ]").
+      { by iFrame "Hlock Hlocked ∗". }
+      wp_pures.
+      by iApply "HΦ".
+    }
+    { (* Case: Query. *)
+      iNamed "Hgcoord".
+      wp_loadField.
+      wp_pures.
+      case_bool_decide as Htseq; wp_pures; last by iApply "HΦ".
+      symmetry in Htseq. inv Htseq.
+      wp_loadField.
+      wp_apply (wp_Mutex__Lock with "Hlock").
+      iIntros "[Hlocked Hgcoord]".
+      iNamed "Hgcoord". iNamed "Hgpp".
+      wp_loadField.
+      wp_pures.
+      wp_loadField.
+      wp_apply (wp_Cond__Signal with "Hcv").
+      wp_loadField.
+      wp_apply (wp_Mutex__Unlock with "[-HΦ]").
+      { by iFrame "Hlock Hlocked ∗". }
+      wp_pures.
+      by iApply "HΦ".
+    }
+    { (* Case: Inquire. *)
+      iNamed "Hgcoord".
+      wp_loadField.
+      wp_pures.
+      case_bool_decide as Htseq; wp_pures; last by iApply "HΦ".
+      symmetry in Htseq. inv Htseq.
+      wp_loadField.
+      wp_apply (wp_Mutex__Lock with "Hlock").
+      iIntros "[Hlocked Hgcoord]".
+      iNamed "Hgcoord". iNamed "Hgpp".
+      do 2 wp_loadField. wp_pures.
+      case_bool_decide; wp_pures; last first.
+      { wp_loadField.
+        wp_apply (wp_Cond__Signal with "Hcv").
+        wp_loadField.
+        wp_apply (wp_Mutex__Unlock with "[-HΦ]").
+        { by iFrame "Hlock Hlocked ∗". }
+        wp_pures.
+        by iApply "HΦ".
+      }
+      wp_loadField. wp_pures.
+      case_bool_decide; wp_pures; last first.
+      { wp_loadField.
+        wp_apply (wp_Cond__Signal with "Hcv").
+        wp_loadField.
+        wp_apply (wp_Mutex__Unlock with "[-HΦ]").
+        { by iFrame "Hlock Hlocked ∗". }
+        wp_pures.
+        by iApply "HΦ".
+      }
+      wp_loadField. wp_pures.
+      case_bool_decide; wp_pures; last first.
+      { wp_loadField.
+        wp_apply (wp_Cond__Signal with "Hcv").
+        wp_loadField.
+        wp_apply (wp_Mutex__Unlock with "[-HΦ]").
+        { by iFrame "Hlock Hlocked ∗". }
+        wp_pures.
+        by iApply "HΦ".
+      }
+      inv H.
+      assert (cid0 = cid) as ->.
+      { destruct cid0 as [r0 g0].
+        destruct cid as [r g].
+        simpl in H0, H3. by subst.
+      }
+      iNamed "Hresp".
+      wp_apply (wp_BackupGroupPreparer__processInquireResult with "Hpwrs Hsafe Hinv Hgpp").
+      { apply Hrk. }
+      { apply Hrid. }
+      { apply Hgid. }
+      iIntros "Hgpp".
+      wp_loadField.
+      wp_apply (wp_Cond__Signal with "Hcv").
+      wp_loadField.
+      wp_apply (wp_Mutex__Unlock with "[-HΦ]").
+      { by iFrame "Hlock Hlocked ∗". }
+      wp_pures.
+      by iApply "HΦ".
+    }
+    { (* Case: Commit. *)
+      iNamed "Hgcoord".
+      wp_loadField.
+      wp_pures.
+      case_bool_decide as Htseq; wp_pures; last by iApply "HΦ".
+      symmetry in Htseq. inv Htseq.
+      wp_loadField.
+      wp_apply (wp_Mutex__Lock with "Hlock").
+      iIntros "[Hlocked Hgcoord]".
+      iNamed "Hgcoord". iNamed "Hgpp".
+      wp_loadField.
+      wp_pures.
+      wp_apply (wp_BackupGroupPreparer__processFinalizationResult with "Hgpp").
+      iIntros "Hgpp".
+      wp_loadField.
+      wp_apply (wp_Cond__Signal with "Hcv").
+      wp_loadField.
+      wp_apply (wp_Mutex__Unlock with "[-HΦ]").
+      { by iFrame "Hlock Hlocked ∗". }
+      wp_pures.
+      by iApply "HΦ".
+    }
+    { (* Case: Abort. *)
+      iNamed "Hgcoord".
+      wp_loadField.
+      wp_pures.
+      case_bool_decide as Htseq; wp_pures; last by iApply "HΦ".
+      symmetry in Htseq. inv Htseq.
+      wp_loadField.
+      wp_apply (wp_Mutex__Lock with "Hlock").
+      iIntros "[Hlocked Hgcoord]".
+      iNamed "Hgcoord". iNamed "Hgpp".
+      wp_loadField.
+      wp_pures.
+      wp_apply (wp_BackupGroupPreparer__processFinalizationResult with "Hgpp").
+      iIntros "Hgpp".
+      wp_loadField.
+      wp_apply (wp_Cond__Signal with "Hcv").
+      wp_loadField.
+      wp_apply (wp_Mutex__Unlock with "[-HΦ]").
+      { by iFrame "Hlock Hlocked ∗". }
+      wp_pures.
+      by iApply "HΦ".
+    }
+  Qed.
+
+End program.
