src/program_proof/tulip/program/util/decode_prepare_proposal.v
@@ -1,0 +1,36 @@
+From Perennial.program_proof.tulip.program Require Import prelude.
+From Perennial.program_proof Require Import marshal_stateless_proof.
+
+Section program.
+  Context `{!heapGS Σ, !paxos_ghostG Σ}.
+
+  Theorem wp_DecodePrepareProposal (bsP : Slice.t) (pp : ppsl) (bstail : list u8) :
+    {{{ own_slice_small bsP byteT (DfracOwn 1) (encode_ppsl pp ++ bstail) }}}
+      DecodePrepareProposal (to_val bsP)
+    {{{ (dataP : Slice.t), RET (ppsl_to_val pp, (to_val dataP));
+        own_slice_small dataP byteT (DfracOwn 1) bstail
+    }}}.
+  Proof.
+    iIntros (Φ) "Hbs HΦ".
+    wp_rec.
+
+    (*@ func DecodePrepareProposal(bs []byte) (tulip.PrepareProposal, []byte) { @*)
+    (*@     rank, bs1 := marshal.ReadInt(bs)                                    @*)
+    (*@     prepared, data := marshal.ReadBool(bs1)                             @*)
+    (*@     pp := tulip.PrepareProposal{                                        @*)
+    (*@         Rank     : rank,                                                @*)
+    (*@         Prepared : prepared,                                            @*)
+    (*@     }                                                                   @*)
+    (*@     return pp, data                                                     @*)
+    (*@ }                                                                       @*)
+    rewrite /encode_ppsl -app_assoc.
+    wp_apply (wp_ReadInt with "Hbs").
+    iIntros (bs1P) "Hbs".
+    wp_apply (wp_ReadBool with "Hbs").
+    iIntros (b dataP) "[%Hb Hdata]".
+    wp_pures.
+    rewrite /ppsl_to_val.
+    by case_bool_decide; subst b; destruct pp.2; try word; iApply "HΦ".
+  Qed.
+
+End program.
